extraction/Types.ml
@@ -3,5 +3,9 @@ type ty =
 | TyBool
 | TyInt
 | TyReal
+| TyQBool
+| TyQInt
+| TyQReal
 | TyString
 | TyVoid
+| TyArray of ty * int * int
