extraction/Values.ml
@@ -1,10 +1,18 @@
 open QArith_base
 open Types
 
+type quality =
+| QGood
+| QBad
+| QUncertain
+
 type value =
 | VBool of bool
 | VInt of int
 | VReal of coq_Q
+| VQBool of bool * quality
+| VQInt of int * quality
+| VQReal of coq_Q * quality
 | VString of char list
 | VVoid
 
@@ -14,9 +22,13 @@ let typeof = function
 | VBool _ -> TyBool
 | VInt _ -> TyInt
 | VReal _ -> TyReal
+| VQBool (_, _) -> TyQBool
+| VQInt (_, _) -> TyQInt
+| VQReal (_, _) -> TyQReal
 | VString _ -> TyString
 | VVoid -> TyVoid
 
 (* has_type : logical inductive *)
-(* with constructors : T_Bool T_Int T_Real T_String T_Void *)
+(* with constructors : T_Bool T_Int T_Real T_QBool T_QInt T_QReal T_String
+   T_Void *)
 
